Well, just added two versions

code/ecdsap256/Hacl.Impl.P256.Ext.fst
@@ -25,7 +25,7 @@ open FStar.Mul
 
 (** 
 The function takes as input a point as a buffer of uint64.
-It moves the point out of domain, normalises it and writes it down to a uint8 buffer.
+It normalises the point and writes it down to a uint8 buffer.
 I think. 
 **)
 
@@ -44,5 +44,30 @@ let point_to_bin p result tempBuffer =
   norm p p tempBuffer;
     let h1 = ST.get() in 
   let isPointAtInfinityResult = isPointAtInfinityPrivate p in 
+  fromFormPoint p result; 
+  isPointAtInfinityResult
+
+
+(** 
+The function takes as input a point as a buffer of uint64.
+It moves it out of domaine, normalises the point and writes it down to a uint8 buffer.
+Disclaimer: I am not sure whether the function is useful, but let it stay. 
+**)
+
+val point_to_bin_2: p: point -> result: lbuffer uint8 (size 64) -> tempBuffer: lbuffer uint64 (size 88) ->
+  Stack uint64 
+  (requires fun h -> live h p /\ live h result /\ live h tempBuffer /\ disjoint tempBuffer p /\ disjoint p result /\
+    point_x_as_nat h p < prime /\
+    point_y_as_nat h p < prime /\
+    point_z_as_nat h p < prime)
+  (ensures fun h0 _ h1 -> modifies (loc p |+| loc result |+| loc tempBuffer) h0 h1)
+
+
+let point_to_bin_2 p result tempBuffer = 
+    let h0 = ST.get() in 
+  norm p p tempBuffer;
+    let h1 = ST.get() in 
+  let isPointAtInfinityResult = isPointAtInfinityPrivate p in 
+  pointFromDomain p p;
   fromFormPoint p result; 
   isPointAtInfinityResult
